some proofs

auto_generated/isabelle/Byte_sequence.thy
@@ -26,7 +26,7 @@ begin
 (*open import Show*)
 
 datatype byte_sequence =
-  Sequence "  word 8 list "
+  Sequence "  8 word list "
 
 (*val acquire_byte_list : string -> error (list byte)*)
 
@@ -42,14 +42,14 @@ definition empty  :: " byte_sequence "  where
 
 
 (*val read_char : byte_sequence -> error (byte * byte_sequence)*)
-fun read_char  :: " byte_sequence \<Rightarrow>( word 8*byte_sequence)error "  where 
+fun read_char  :: " byte_sequence \<Rightarrow>( 8 word*byte_sequence)error "  where 
      " read_char (Sequence([])) = ( error_fail (''read_char: sequence is empty''))"
 |" read_char (Sequence(x # xs)) = ( error_return (x, Sequence xs))" 
 declare read_char.simps [simp del]
 
 
 (*val repeat : natural -> byte -> list byte*)
-function (sequential,domintros)  repeat  :: " nat \<Rightarrow> word 8 \<Rightarrow>( word 8)list "  where 
+function (sequential,domintros)  repeat  :: " nat \<Rightarrow> 8 word \<Rightarrow>( 8 word)list "  where 
      " repeat count1 c = (
   (case  count1 of
       0 => []
@@ -57,9 +57,11 @@ function (sequential,domintros)  repeat  :: " nat \<Rightarrow> word 8 \<Rightar
   ))" 
 by pat_completeness auto
 
+termination by lexicographic_order
+
 
 (*val create : natural -> byte -> byte_sequence*)
-definition create  :: " nat \<Rightarrow> word 8 \<Rightarrow> byte_sequence "  where 
+definition create  :: " nat \<Rightarrow> 8 word \<Rightarrow> byte_sequence "  where 
      " create count1 c = (
   Sequence (repeat count1 c))"
 
@@ -86,9 +88,10 @@ function (sequential,domintros)  concat_byte_sequence  :: "(byte_sequence)list \
       ))" 
 by pat_completeness auto
 
+termination by lexicographic_order
 
 (*val from_byte_lists : list (list byte) -> byte_sequence*)
-definition from_byte_lists  :: "(( word 8)list)list \<Rightarrow> byte_sequence "  where 
+definition from_byte_lists  :: "(( 8 word)list)list \<Rightarrow> byte_sequence "  where 
      " from_byte_lists ts = (
   Sequence (List.concat ts))"
 
@@ -129,6 +132,8 @@ function (sequential,domintros)  dropbytes  :: " nat \<Rightarrow> byte_sequence
   ))" 
 by pat_completeness auto
 
+termination by lexicographic_order
+
 
 (*val takebytes : natural -> byte_sequence -> error byte_sequence*)
 function (sequential,domintros)  takebytes  :: " nat \<Rightarrow> byte_sequence \<Rightarrow>(byte_sequence)error "  where 
@@ -148,9 +153,11 @@ function (sequential,domintros)  takebytes  :: " nat \<Rightarrow> byte_sequence
   ))" 
 by pat_completeness auto
 
+termination by lexicographic_order
+
 
 (*val read_2_bytes_le : byte_sequence -> error ((byte * byte) * byte_sequence)*)
-definition read_2_bytes_le  :: " byte_sequence \<Rightarrow>(( word 8* word 8)*byte_sequence)error "  where 
+definition read_2_bytes_le  :: " byte_sequence \<Rightarrow>(( 8 word* 8 word)*byte_sequence)error "  where 
      " read_2_bytes_le bs0 = (
   read_char bs0 >>= (\<lambda> (b0, bs1) . 
   read_char bs1 >>= (\<lambda> (b1, bs2) . 
@@ -158,7 +165,7 @@ definition read_2_bytes_le  :: " byte_sequence \<Rightarrow>(( word 8* word 8)*b
 
 
 (*val read_2_bytes_be : byte_sequence -> error ((byte * byte) * byte_sequence)*)
-definition read_2_bytes_be  :: " byte_sequence \<Rightarrow>(( word 8* word 8)*byte_sequence)error "  where 
+definition read_2_bytes_be  :: " byte_sequence \<Rightarrow>(( 8 word* 8 word)*byte_sequence)error "  where 
      " read_2_bytes_be bs0 = (
   read_char bs0 >>= (\<lambda> (b0, bs1) . 
   read_char bs1 >>= (\<lambda> (b1, bs2) . 
@@ -166,7 +173,7 @@ definition read_2_bytes_be  :: " byte_sequence \<Rightarrow>(( word 8* word 8)*b
 
 
 (*val read_4_bytes_le : byte_sequence -> error ((byte * byte * byte * byte) * byte_sequence)*)
-definition read_4_bytes_le  :: " byte_sequence \<Rightarrow>(( word 8* word 8* word 8* word 8)*byte_sequence)error "  where 
+definition read_4_bytes_le  :: " byte_sequence \<Rightarrow>(( 8 word* 8 word* 8 word* 8 word)*byte_sequence)error "  where 
      " read_4_bytes_le bs0 = (
   read_char bs0 >>= (\<lambda> (b0, bs1) . 
   read_char bs1 >>= (\<lambda> (b1, bs2) . 
@@ -176,7 +183,7 @@ definition read_4_bytes_le  :: " byte_sequence \<Rightarrow>(( word 8* word 8* w
 
 
 (*val read_4_bytes_be : byte_sequence -> error ((byte * byte * byte * byte) * byte_sequence)*)
-definition read_4_bytes_be  :: " byte_sequence \<Rightarrow>(( word 8* word 8* word 8* word 8)*byte_sequence)error "  where 
+definition read_4_bytes_be  :: " byte_sequence \<Rightarrow>(( 8 word* 8 word* 8 word* 8 word)*byte_sequence)error "  where 
      " read_4_bytes_be bs0 = (
   read_char bs0 >>= (\<lambda> (b0, bs1) . 
   read_char bs1 >>= (\<lambda> (b1, bs2) . 
@@ -186,7 +193,7 @@ definition read_4_bytes_be  :: " byte_sequence \<Rightarrow>(( word 8* word 8* w
 
 
 (*val read_8_bytes_le : byte_sequence -> error ((byte * byte * byte * byte * byte * byte * byte * byte) * byte_sequence)*)
-definition read_8_bytes_le  :: " byte_sequence \<Rightarrow>(( word 8* word 8* word 8* word 8* word 8* word 8* word 8* word 8)*byte_sequence)error "  where 
+definition read_8_bytes_le  :: " byte_sequence \<Rightarrow>(( 8 word* 8 word* 8 word* 8 word* 8 word* 8 word* 8 word* 8 word)*byte_sequence)error "  where 
      " read_8_bytes_le bs0 = (
   read_char bs0 >>= (\<lambda> (b0, bs1) . 
   read_char bs1 >>= (\<lambda> (b1, bs2) . 
@@ -200,7 +207,7 @@ definition read_8_bytes_le  :: " byte_sequence \<Rightarrow>(( word 8* word 8* w
 
 
 (*val read_8_bytes_be : byte_sequence -> error ((byte * byte * byte * byte * byte * byte * byte * byte) * byte_sequence)*)
-definition read_8_bytes_be  :: " byte_sequence \<Rightarrow>(( word 8* word 8* word 8* word 8* word 8* word 8* word 8* word 8)*byte_sequence)error "  where 
+definition read_8_bytes_be  :: " byte_sequence \<Rightarrow>(( 8 word* 8 word* 8 word* 8 word* 8 word* 8 word* 8 word* 8 word)*byte_sequence)error "  where 
      " read_8_bytes_be bs0 = (
   read_char bs0 >>= (\<lambda> (b0, bs1) . 
   read_char bs1 >>= (\<lambda> (b1, bs2) . 
