auto_generated/isabelle/Elf_Roundtrip_Proofs.thy
@@ -2,6 +2,97 @@ theory
   Elf_Roundtrip_Proofs
 imports
   Main
-  Elf_executable_file
+  Elf_file
 begin
+
+  section {* Error monad properties *}
+
+  lemma error_return_bind_neutral1 [simp]:
+    shows "error_return x >>= f = f x"
+  unfolding error_return_def by (simp add: error_bind.simps)
+
+  lemma error_return_bind_neutral2 [simp]: 
+    shows "x >>= error_return = x"
+  by(cases x, simp_all, auto simp add: error_bind.simps error_return_def)
+
+  lemma error_bind_compose [simp]:
+    shows "(x >>= f) >>= g = x >>= (\<lambda>y. f y >>= g)"
+  by(cases x, simp_all, auto simp add: error_bind.simps)
+
+  lemma error_bind_case [simp]:
+    fixes x :: "'a error" and f :: "'a \<Rightarrow> 'b error"
+    shows "x >>= (\<lambda>r. f r) = (case x of Success r \<Rightarrow> f r | Fail e \<Rightarrow> Fail e)"
+  by(cases x, simp_all, auto simp add: error_bind.simps)
+
+  lemma repeatM_length [simp]:
+    fixes m :: "nat" and act :: "'a error"
+    assumes "repeatM m act = Success r"
+    shows "List.length r = m"
+  sorry
+
+  lemma repeatM'_length [simp]:
+    fixes m :: "nat" and e :: "'a" and f :: "'a \<Rightarrow> ('b \<times> 'a) error" and r :: "'b list" and rest :: "'a"
+    assumes "repeatM' m e f = Success (r, rest)"
+    shows "List.length r = m"
+  sorry
+  
+  lemma mapM_length [simp]:
+    fixes f :: "'a \<Rightarrow> 'b error" and i :: "'a list" and r :: "'b list"
+    assumes "mapM f i = Success r"
+    shows "List.length r = List.length i"
+  sorry
+
+  lemma mapM_error_return [simp]:
+    fixes i :: "'a list"
+    shows "mapM error_return i = Success i"
+  proof(induct i)
+    case Nil
+      have "mapM error_return [] = error_return []" by simp
+      moreover have "... = Success []" using error_return_def by fastforce
+      ultimately show ?case by auto
+  next
+    case (Cons x xs)
+      assume *: "mapM error_return xs = Success xs"
+      have "mapM error_return (x#xs) =
+        error_return x >>= (\<lambda>h. mapM error_return xs >>= (\<lambda>t. error_return (h#t)))" by simp
+      moreover have "... = mapM error_return xs >>= (\<lambda>t. error_return (x#t))" using error_return_def error_bind.simps by metis
+      moreover have "... = Success xs >>= (\<lambda>t. error_return (x#t))" using * by simp
+      moreover have "...  = error_return (x#xs)" using error_bind.simps by auto
+      moreover have "... = Success (x#xs)" using error_return_def by metis
+      ultimately show ?case by auto
+  qed
+
+  section {* Helpful lemmas *}
+
+  lemma elf64_header_out_in_roundtrip:
+    fixes hdr64 :: "elf64_header" and bs :: "byte_sequence"
+    shows "read_elf64_header (bytes_of_elf64_header hdr64) = Success (hdr64, bs)"
+  sorry
+
+  section {* The main roundtripping theorems *}
+
+  theorem elf64_out_in_roundtrip:
+    fixes ef64 :: "elf64_file" and bs :: "byte_sequence"
+    assumes "bytes_of_elf64_file ef64 = Success bs"
+    shows "read_elf64_file bs = Success ef64"
+  sorry
+
+  theorem elf64_in_out_roundtrip:
+    fixes ef64 :: "elf64_file" and bs :: "byte_sequence"
+    assumes "read_elf64_file bs = Success ef64"
+    shows "bytes_of_elf64_file ef64 = Success bs"
+  sorry
+
+  theorem elf32_out_in_roundtrip:
+    fixes ef32 :: "elf32_file" and bs :: "byte_sequence"
+    assumes "bytes_of_elf32_file ef32 = Success bs"
+    shows "read_elf32_file bs = Success ef64"
+  sorry
+
+  theorem elf32_in_out_roundtrip:
+    fixes ef32 :: "elf32_file" and bs :: "byte_sequence"
+    assumes "read_elf32_file bs = Success ef32"
+    shows "bytes_of_elf32_file ef32 = Success bs"
+  sorry
+
 end
